io/Model.fst
@@ -4,47 +4,48 @@ open FStar.List.Tot
 open FStar.Calc
 open FStar.Tactics
 
-
 open Free.IO
 open Common
 open ExtraTactics
-open TC.Checkable
+open TC.Monitorable
 open DM
 open Instrument
 
 noeq type model_type = {
   interface : Type;
-  set_of_traces : Type -> Type;
-  monitorable_prop : Type;
+  monitor : interface -> Type;
 
-  prog_s  : interface -> monitorable_prop -> Type;
-  ctx_s   : interface -> monitorable_prop -> Type;
-  whole_s : interface -> monitorable_prop -> Type;
-  link_s  : (#i:interface) -> (#pi:monitorable_prop) ->
-            ctx_s i pi -> prog_s i pi -> Tot (whole_s i pi);
+  prog_s  : i:interface -> monitor i -> Type;
+  ctx_s   : i:interface -> monitor i -> Type;
+  whole_s : i:interface -> monitor i -> Type;
+  link_s  : (#i:interface) -> (#m:monitor i) ->
+            ctx_s i m -> prog_s i m -> Tot (whole_s i m);
 
-  prog_t  : interface -> monitorable_prop -> Type;
+  prog_t  : i:interface -> monitor i -> Type;
   ctx_t   : interface -> Type;
-  ictx_t   : interface -> monitorable_prop -> Type;
+  ictx_t   : i:interface -> monitor i -> Type;
   whole_t : interface -> Type;
-  link_t  : (#i:interface) -> (#pi:monitorable_prop) ->
-            ctx_t i -> prog_t i pi -> Tot (whole_t i);
+  link_t  : (#i:interface) -> (#m:monitor i) ->
+            ctx_t i -> prog_t i m -> Tot (whole_t i);
 
-  instrument : (#i:interface) -> (#pi:monitorable_prop) ->
-               ctx_t i -> ictx_t i pi;
+  instrument : (#i:interface) -> (#m:monitor i) ->
+               ctx_t i -> ictx_t i m;
 
-  compile_prog  : (#i:interface) -> (#pi:monitorable_prop) ->
-                  prog_s i pi -> Tot (prog_t i pi);
+  compile_prog  : (#i:interface) -> (#m:monitor i) ->
+                  prog_s i m -> Tot (prog_t i m);
 }
 
 noeq type interface = {
   ctx_arg : Type;
   ctx_ret : Type;
-  ctx_post :
-    ctx_arg -> trace -> r:(maybe ctx_ret) -> trace -> b:Type0{r == Inr Contract_failure ==> b};
-  ctx_post_c : checkable4 ctx_post;
-
   ret : Type;
+}
+
+noeq type monitor (i:interface) = {
+  pi : monitorable_prop;
+  pre : i.ctx_arg -> trace -> Type0;
+  post : i.ctx_arg -> trace -> r:(maybe i.ctx_ret) -> trace -> b:Type0{r == Inr Contract_failure ==> b};
+  post_c : monitorable_post pre post pi;
 }
 
 (** The whole program does not need a pre-condition. 
@@ -58,11 +59,8 @@ let whole_pre' _ h = true
 val whole_pre : unit -> trace -> Type0
 let whole_pre x h = whole_pre' x h
 
-let whole_pre_cc : checkable2 whole_pre =
-  general_is_checkable2 unit trace whole_pre'
-
-type whole_s (i:interface) (pi:monitorable_prop) =
-  x:unit -> IIO i.ret pi (whole_pre x) (fun _ _ _ -> True)
+type whole_s (i:interface) (m:monitor i) =
+  x:unit -> IIO i.ret m.pi (whole_pre x) (fun _ _ _ -> True)
 type whole_t (i:interface) = unit -> MIIO (maybe i.ret)
 
 (** Having a pre-condition for the context is not necessary,
@@ -86,35 +84,35 @@ We make the following remarks about a context's post-condition:
 let tpre : (i:interface) -> (i.ctx_arg -> trace -> bool) = fun i x h -> true
 type ctx_t (i:interface) = i.ctx_arg -> MIO i.ctx_ret
 
-type ictx_t (i:interface) (pi:monitorable_prop) =
-  (x:i.ctx_arg) -> IIO (maybe i.ctx_ret) pi (fun h -> tpre i x h) (fun _ _ _ -> True)
+type ictx_t (i:interface) (m:monitor i) =
+  (x:i.ctx_arg) -> IIO (maybe i.ctx_ret) m.pi (fun h -> tpre i x h) (fun _ _ _ -> True)
 (** The ctx_s stands for the instrumented context, therefore the
     output type is different compared to ctx_t.
     ctx_t has the output type `i.ctx_ret`, but ctx_s has `maybe i.ctx_ret`.
     This is needed to accomodate the possibility of failure during 
     instrumentation when a contract is violated. **)
-type ctx_s (i:interface) (pi:monitorable_prop) =
-  (x:i.ctx_arg) -> IIO (maybe i.ctx_ret) pi (fun h -> tpre i x h) (i.ctx_post x)
+type ctx_s (i:interface) (m:monitor i) =
+  (x:i.ctx_arg) -> IIO (maybe i.ctx_ret) m.pi (m.pre x) (m.post x)
 
 (** The partial program does not need a pre- or a post-condition because
     it is the starting point of the execution in this model. **)
-type prog_s (i:interface) (pi:monitorable_prop) =
-  ctx_s i pi -> IIO i.ret pi (fun _ -> True) (fun _ _ _ -> True)
+type prog_s (i:interface) (m:monitor i) =
+  ctx_s i m -> IIO i.ret m.pi (fun _ -> True) (fun _ _ _ -> True)
 (** compared to prog_s, prog_t can fail because it has to check the
     history with which it starts. prog_t is prog_s wrapped in a new 
     function which adds a runtime check for verifying if pi was 
     respected until now **)
-type prog_t (i:interface) (pi:monitorable_prop) =
-  ictx_t i pi -> MIIO (maybe i.ret)
+type prog_t (i:interface) (m:monitor i) =
+  ictx_t i m -> MIIO (maybe i.ret)
 
 let instrument
-  (#i  : interface)
-  (#pi : monitorable_prop)
+  (#i : interface)
+  (#m : monitor i)
   (ct : ctx_t i) :
-  Tot (ictx_t i pi) =
+  Tot (ictx_t i m) =
     fun x ->
       instrument_MIIO
-        (cast_io_iio ((* MIIO.*)reify (ct x) [] (fun _ _ -> True))) pi
+        (cast_io_iio ((* MIIO.*)reify (ct x) [] (fun _ _ -> True))) m.pi
  
 let extract_local_trace (h':trace) (pi:monitorable_prop) :
   IIO trace pi
@@ -134,17 +132,19 @@ let extract_local_trace (h':trace) (pi:monitorable_prop) :
 
 let enforce_post
   (#i:interface)
-  (#pi:monitorable_prop)
-  (f:i.ctx_arg -> IIO (maybe i.ctx_ret) pi (fun _ -> True) (fun _ _ _ -> true))
+  (#m:monitor i)
+  (f:i.ctx_arg -> IIO (maybe i.ctx_ret) (m.pi) (fun _ -> True) (fun _ _ _ -> True))
   (x:i.ctx_arg) :
-  IIO (maybe i.ctx_ret) pi (fun _ -> True) (i.ctx_post x)  =
+  IIO (maybe i.ctx_ret) m.pi (m.pre x) (m.post x) =
   let h = get_trace () in
   let r : maybe i.ctx_ret = f x in
   Classical.forall_intro (lemma_suffixOf_append h);
-  let lt = extract_local_trace h pi in
+  let lt = extract_local_trace h m.pi in
   Classical.forall_intro_2 (Classical.move_requires_2 (lemma_append_rev_inv_tail h));
-  if i.ctx_post_c.check4 x h r lt then r
-  else Inr Contract_failure
+  if m.post_c.result_check x h r lt then begin
+    assume (enforced_globally m.pi ((rev lt)@h) ==> enforced_locally m.pi h lt);
+    r
+  end else Inr Contract_failure
 
 (**
   Context: During compilation, p is wrapped in a new function
@@ -169,32 +169,29 @@ let enforce_post
 **)
 
 let compile_prog
-  (#i  : interface)
-  (#pi : monitorable_prop)
-  (p  : prog_s i pi) :
-  Tot (prog_t i pi) =
+  (#i : interface)
+  (#m : monitor i)
+  (p  : prog_s i m) :
+  Tot (prog_t i m) =
   _IIOwp_as_MIIO
-    (fun _ -> iio_pre pi)
-    (fun _ h r lt -> iio_post pi h r lt)
-    (fun (ict:ictx_t i pi) -> p (enforce_post #i #pi ict))
+    (fun _ -> iio_pre m.pi)
+    (fun _ h r lt -> iio_post m.pi h r lt)
+    (fun (ict:ictx_t i m) -> p (enforce_post #i #m ict))
 
-val link_s  : (#i:interface) -> (#pi:monitorable_prop) -> ctx_s i pi ->
-              prog_s i pi -> Tot (whole_s i pi)
+val link_s  : (#i:interface) -> (#m:monitor i) -> ctx_s i m ->
+              prog_s i m -> Tot (whole_s i m)
 let link_s = (fun #i #pi c p -> (fun _ -> p c))
 
 (** during linking, p expects a context of type ctx_s, but link_t 
 gets a context of type ctx_t, therefore, the linker must instrument 
 the context. **)
-val link_t  : (#i:interface) -> (#pi:monitorable_prop) -> ctx_t i ->
-              prog_t i pi -> Tot (whole_t i)
-let link_t #i #pi c p : whole_t i = (fun _ -> p (instrument #i #pi c))
-
-type set_of_traces (a:Type) = trace * a -> Type0
+val link_t  : (#i:interface) -> (#m:monitor i) -> ctx_t i ->
+              prog_t i m -> Tot (whole_t i)
+let link_t #i #m c p : whole_t i = (fun _ -> p (instrument #i #m c))
 
 let model : model_type = { 
   interface = interface;
-  set_of_traces = set_of_traces;
-  monitorable_prop = monitorable_prop;
+  monitor = monitor;
 
   prog_s  = prog_s;
   ctx_s   = ctx_s;
