io/case-studies/case-study-1/Linker.fst
@@ -6,10 +6,10 @@ open WebServer
 open Plugin
 open TC.MLify.MIIO
 
-let compiled_webserver = comp.compile_prog #i #pi webserver
+let compiled_webserver = model.compile_prog #i #m webserver
 
-let whole : comp.whole_t i = 
-  comp.link_t #i #pi plugin compiled_webserver
+let whole : model.whole_t i = 
+  model.link_t #i #m plugin compiled_webserver
 
 let whole_ML = mlify #_ #(mlifyable_miio _ _) whole
 
