io/TC.Monitorable.fst
@@ -1,0 +1,17 @@
+module TC.Monitorable
+
+open FStar.Tactics
+open FStar.Tactics.Typeclasses
+
+open Free.IO
+
+class monitorable_post (#t1:Type) (#t2:Type) 
+  (pre : t1 -> trace -> Type0)
+  (post : t1 -> trace -> t2 -> trace -> Type0)
+  (pi : monitorable_prop) = {
+  result_check : t1 -> trace -> t2 -> trace -> bool;
+  (** this condition makes sure that all trace properties enforced by post are instrumented by pi **)
+  c1post : squash (forall x h lt. pre x h /\ enforced_locally pi h lt ==> (exists r. post x h r lt));
+  (** this one makes sure that the post at the end is enough **)
+  c2post: squash (forall x h r lt. pre x h /\ enforced_locally pi h lt /\ result_check x h r lt ==> post x h r lt)
+}
