io/case-studies/case-study-2/WebServer.Compiled.fst
@@ -12,8 +12,8 @@ open TC.MLify.MIIO
 open WebServer
 
 (** TODO: can these two steps be combined? **)
-let compiled_webserver : prog_t i pi = model.compile_prog #i #pi webserver
+let compiled_webserver : prog_t i m = model.compile_prog #i #m webserver
 let compiled_webserver'' : (Types.file_descr -> Tot (maybe unit)) -> ML (maybe unit) =
   (mlify #_
-    #(mlifyable_iio_miio file_descr (maybe unit) (maybe unit) pi #TC.Export.ml_file_descr)
+    #(mlifyable_iio_miio file_descr (maybe unit) (maybe unit) m.pi #TC.Export.ml_file_descr)
     compiled_webserver)
